LogicalRefinement/Stlc/InterpSubst.lean
@@ -2,6 +2,7 @@ import LogicalRefinement.Untyped
 import LogicalRefinement.Typed
 import LogicalRefinement.Stlc.Basic
 import LogicalRefinement.Stlc.Interp
+import LogicalRefinement.Stlc.InterpWk
 import LogicalRefinement.Stlc.Subst
 import LogicalRefinement.Utils
 open Annot
