LogicalRefinement/Stlc/InterpWk.lean
@@ -2,18 +2,36 @@ import LogicalRefinement.Untyped
 import LogicalRefinement.Typed
 import LogicalRefinement.Stlc.Basic
 import LogicalRefinement.Stlc.Interp
-import LogicalRefinement.Stlc.InterpSubst
 import LogicalRefinement.Stlc.Subst
 open Annot
 open AnnotSort
 
-theorem Term.wk_stlc_commute {Γ Δ ρ a} 
-  (H: Δ ⊢ a: term A) 
+theorem Term.wk_stlc_commute {Γ Δ ρ}
+  (a: Term)
   (R: WkCtx ρ Γ Δ)
   : (a.wk ρ).stlc
   = a.stlc.wk ρ
   := by {
-    rw [<-Subst.subst_wk_compat]
-    rw [<-Stlc.Subst.subst_wk_compat]
-    exact Term.term_subst_stlc_commute H R.to_subst
+    induction a generalizing ρ Γ Δ with
+    | var => rfl
+    | const c => cases c <;> rfl
+    | unary k t I => 
+      (cases k <;> try rfl)
+      rename Fin 2 => b;
+      match b with
+      | 0 => dsimp only [stlc]; rw [I R]; rfl
+      | 1 => dsimp only [stlc]; rw [I R]; rfl
+    | _ => 
+      rename TermKind _ => k;
+      rename_i' I0 I1 I2 I3 I4;
+      cases k <;>
+      (try rename AnnotSort => k <;> cases k) <;>
+      dsimp only [stlc, Stlc.wk, Wk.liftn] <;>
+      simp only [Term.stlc_ty_wk] <;>
+      (try rw [I0]) <;>
+      (try rw [I1]) <;>
+      (try rw [I2]) <;>
+      (try rw [I3]) <;>
+      (try rw [I4]) <;>
+      repeat first | assumption | constructor
   }
